fixed PingPong

Test/civl/inductive-sequentialization/PingPong.bpl
@@ -16,169 +16,45 @@ type ChannelId;
 
 // The following global variables models all instances of a bidirectional channel indexed
 // the ChannelId type. A single instance of PingPong will only use a single channel id.
-var {:layer 0,3} channel: [ChannelId]ChannelPair;
+var {:layer 0,1} channel: [ChannelId]ChannelPair;
 
 // The id of a bidirectional channel can be split into two permissions---Left and Right.
 // Left permission is used to receive from the left channel and send to the right channel.
 // Right permission is used to receive from the right channel and send to the left channel.
 datatype ChannelHandle { Left(cid: ChannelId), Right(cid: ChannelId) }
 
-function {:inline} BothHandles(cid: ChannelId): Set ChannelHandle {
-  Set_Add(Set_Singleton(Left(cid)), Right(cid))
-}
+function {:inline} BothHandles(cid: ChannelId): Set ChannelHandle
+{ Set_Add(Set_Singleton(Left(cid)), Right(cid)) }
 
-function {:inline} EmptyChannel () : [int]int
-{ MapConst(0) }
+function {:inline} Empty() : [int]int { MapConst(0) }
 
-////////////////////////////////////////////////////////////////////////////////
-
-atomic action {:layer 3}
-MAIN' (cid: ChannelId, {:linear_in} handles: Set ChannelHandle)
-{
-  assert handles == BothHandles(cid);
-  assert channel[cid] == ChannelPair(EmptyChannel(), EmptyChannel());
-}
-
-action {:layer 2}
-INV (cid: ChannelId, {:linear_in} handles: Set ChannelHandle)
-creates PING, PONG;
-modifies channel;
-{
-  var {:linear} handles': Set ChannelHandle;
-  var {:linear} left: One ChannelHandle;
-  var {:linear} right: One ChannelHandle;
-  var {:pool "INV"} c: int;
-
-  assert handles == BothHandles(cid);
-  assert channel[cid] == ChannelPair(EmptyChannel(), EmptyChannel());
-
-  assume {:add_to_pool "INV", 0, c, c+1} 0 < c;
-  handles' := handles;
-  call left := One_Get(handles', Left(cid));
-  call right := One_Get(handles', Right(cid));
-  if (*) {
-    channel[cid] := ChannelPair(EmptyChannel(), EmptyChannel()[c := 1]);
-    async call PONG(c, right);
-    async call PING(c, left);
-    call set_choice(PONG(c, right));
-  } else if (*) {
-    channel[cid] := ChannelPair(EmptyChannel(), EmptyChannel()[0 := 1]);
-    async call PONG(c, right);
-    call set_choice(PONG(c, right));
-  } else if (*) {
-    channel[cid] := ChannelPair(EmptyChannel()[c := 1], EmptyChannel());
-    async call PONG(c+1, right);
-    async call PING(c, left);
-    call set_choice(PING(c, left));
-  } else {
-    channel[cid] := ChannelPair(EmptyChannel(), EmptyChannel());
-  }
-}
+function {:inline} Singleton(x: int): [int]int { Empty()[x := 1] }
 
 ////////////////////////////////////////////////////////////////////////////////
 
-atomic action {:layer 2}
-MAIN (cid: ChannelId, {:linear_in} handles: Set ChannelHandle)
-refines MAIN' using INV;
-creates PING, PONG;
-modifies channel;
-{
-  var {:linear} handles': Set ChannelHandle;
-  var {:linear} left: One ChannelHandle;
-  var {:linear} right: One ChannelHandle;
+yield invariant {:layer 1} YieldMain(cid: ChannelId, {:linear} handles: Set ChannelHandle);
+invariant handles == BothHandles(cid);
+invariant channel[cid] == ChannelPair(Empty(), Empty());
 
-  assert handles == BothHandles(cid);
-  assert channel[cid] == ChannelPair(EmptyChannel(), EmptyChannel());
-  channel[cid] := ChannelPair(EmptyChannel(), EmptyChannel()[1 := 1]);
-  handles' := handles;
-  call left := One_Get(handles', Left(cid));
-  call right := One_Get(handles', Right(cid));
-  async call PING(1, left);
-  async call PONG(1, right);
-}
-
-async atomic action {:layer 2} PING (x: int, {:linear_in} p: One ChannelHandle)
-creates PING;
-modifies channel;
-requires call YieldPing(x, p);
-{
-  var left_channel: [int]int;
-  var right_channel: [int]int;
-
-  left_channel := channel[p->val->cid]->left;
-  right_channel := channel[p->val->cid]->right;
-
-  assert x > 0;
-  assert p->val is Left;
-  assert IsSet(left_channel);
-  assert left_channel[x := 0] == MapConst(0);
-
-  assume left_channel[x] > 0;
-  left_channel[x] := left_channel[x] - 1;
-
-  if (*)
-  {
-    right_channel[x+1] := right_channel[x+1] + 1;
-    async call PING(x+1, p);
-  }
-  else
-  {
-    right_channel[0] := right_channel[0] + 1;
-  }
-  channel[p->val->cid] := ChannelPair(left_channel, right_channel);
-}
-
-async atomic action {:layer 2} PONG (y: int, {:linear_in} p: One ChannelHandle)
-creates PONG;
-modifies channel;
-requires call YieldPong(y, p);
-{
-  var left_channel: [int]int;
-  var right_channel: [int]int;
-
-  left_channel := channel[p->val->cid]->left;
-  right_channel := channel[p->val->cid]->right;
-
-  assert y > 0;
-  assert p->val is Right;
-  assert IsSet(right_channel);
-  assert right_channel[0 := 0] == MapConst(0) || right_channel[y := 0] == MapConst(0);
-
-  if (*)
-  {
-    assume right_channel[y] > 0;
-    right_channel[y] := right_channel[y] - 1;
-    left_channel[y] := left_channel[y] + 1;
-    async call PONG(y+1, p);
-  }
-  else
-  {
-    assume right_channel[0] > 0;
-    right_channel[0] := right_channel[0] - 1;
-  }
-  channel[p->val->cid] := ChannelPair(left_channel, right_channel);
-}
-
-yield invariant {:layer 2} YieldPing (x: int, {:linear} p: One ChannelHandle);
+yield invariant {:layer 1} YieldPing(x: int, {:linear} p: One ChannelHandle);
 invariant p->val is Left;
-invariant (var left_channel := channel[p->val->cid]->left;
-            IsSet(left_channel) &&
-            left_channel[x := 0] == MapConst(0) && left_channel[x] == 1);
-invariant channel[p->val->cid]->right == MapConst(0);
+invariant x > 0;
+invariant (var left_channel, right_channel := channel[p->val->cid]->left, channel[p->val->cid]->right;
+            (left_channel == Empty() && right_channel == Singleton(x) && x > 0) ||
+            (left_channel == Singleton(x) && right_channel == Empty()));
 
-yield invariant {:layer 2} YieldPong (y: int, {:linear} p: One ChannelHandle);
+yield invariant {:layer 1} YieldPong(y: int, {:linear} p: One ChannelHandle);
 invariant p->val is Right;
-invariant (var right_channel := channel[p->val->cid]->right;
-            IsSet(right_channel) &&
-            (right_channel[0] == 1 || right_channel[y] == 1) &&
-            (right_channel[0 := 0] == MapConst(0) || right_channel[y := 0] == MapConst(0)));
-invariant channel[p->val->cid]->left == MapConst(0);
+invariant y > 0;
+invariant (var left_channel, right_channel := channel[p->val->cid]->left, channel[p->val->cid]->right;
+            (left_channel == Empty() && (right_channel == Singleton(y) || right_channel == Singleton(0))) ||
+            (left_channel == Singleton(y-1) && right_channel == Empty()));
 
 ////////////////////////////////////////////////////////////////////////////////
 
 yield procedure {:layer 1}
 main (cid: ChannelId, {:linear_in} handles: Set ChannelHandle)
-refines MAIN;
+requires call YieldMain(cid, handles);
 {
   var {:linear} handles': Set ChannelHandle;
   var {:linear} left: One ChannelHandle;
@@ -194,7 +70,7 @@ refines MAIN;
 
 yield procedure {:layer 1}
 ping (x: int, {:linear_in} p: One ChannelHandle)
-refines PING;
+requires call YieldPing(x, p);
 {
   var x': int;
 
@@ -213,7 +89,7 @@ refines PING;
 
 yield procedure {:layer 1}
 pong (y: int, {:linear_in} p: One ChannelHandle)
-refines PONG;
+requires call YieldPong(y, p);
 {
   var y': int;
 
